fix to the alloca initialization

src/coq/Compiler.v
@@ -163,6 +163,49 @@ Definition load v : EXP local_id :=
 Definition comp cmp v1 v2 : EXP local_id :=
   emit (INSTR_Op (SV (OP_ICmp cmp i64 v1 v2))).
 
+(* initialization monad ----------------------------------------------------- *)
+
+Definition INIT A := ST (int * int * code) (err A).
+
+Definition init_map (A B:Type) (f:A->B) (g:INIT A) : INIT B :=
+  fun s =>
+    let '(st, x) := g s in
+    match x with
+    | inl e  => (st, inl e)
+    | inr a => (st, inr (f a))
+    end.
+
+Instance init_functor : @Functor INIT := init_map.
+
+Definition init_ret (A:Type) (x:A) : INIT A :=
+  fun s => (s, inr x).
+
+Definition init_bind (A B:Type) (g:INIT A) (f:A -> INIT B) : INIT B :=
+  fun s =>
+    let '(st, x) := g s in
+    match x with
+    | inl e => (st, inl e)
+    | inr a => (f a) st
+    end.
+Program Instance init_monad : (@Monad INIT) init_functor := _.
+Next Obligation.
+  split.
+  - exact init_ret.
+  - exact init_bind.
+Defined.    
+
+Instance init_err : (@ExceptionMonad string INIT _ _) := fun _ e => fun s => (s, inl e).
+
+Definition lift_init {A} (e:string) (m:option A) : INIT A :=
+  fun s => (s, trywith e m).
+
+
+Definition alloca : () -> INIT local_id :=
+  fun _ => fun '(n, m, is) =>
+    let lid := lid_of_Z n in
+    let vid := IVoid m in
+    ((1+n, 1+m, ((vid, INSTR_Store false (i64, val_of_nat 0) (i64ptr, local lid) None) :: (IId lid, INSTR_Alloca i64 None None)::is)), mret lid)%Z.
+  
 
 (* 
   Compiler state for commands
@@ -222,6 +265,15 @@ Definition cmd_of_exp {A} (exp : EXP A) : CMD (code * A) :=
     | inr ans => (mk_cs n' m is tm bs, inr (ise, ans))
     end.
 
+Definition cmd_of_init {A} (init : INIT A) : CMD (code * A) :=
+  fun '(mk_cs n m is tm bs) =>
+    let '((n', m', ise), v) := init (n, m, []) in
+    match v with
+    | inl e => (mk_cs n m is tm bs, inl e)
+    | inr ans => (mk_cs n' m' is tm bs, inr (ise, ans))
+    end.
+  
+
 Definition inject_code (ise:code) : CMD () :=
     fun '(mk_cs n m is tm bs) => (mk_cs n m (ise++is) tm bs, mret ()).
 
@@ -233,9 +285,11 @@ Definition emit_cmd instr : CMD local_id :=
     let lid := lid_of_Z n in
     (mk_cs (1+n) m ((IId lid, instr)::is) tm bs, mret lid)%Z.
 
+(*
 Definition alloca : () -> CMD local_id :=
    fun _ => emit_cmd (INSTR_Alloca i64 None None).
-    
+*)  
+  
 Definition emitvoid instr : CMD () :=
     fun '(mk_cs n m is tm bs) =>
       let tid := (IVoid m) in
@@ -367,7 +421,7 @@ Fixpoint compile_com (g:ctxt) (c:com) : CMD () :=
     mret ()    
   end.
 
-Fixpoint compile_fv (l:list id) : CMD ctxt :=
+Fixpoint compile_fv (l:list id) : INIT ctxt :=
   match l with
   | [] => mret empty
   | x::xs =>
@@ -376,7 +430,7 @@ Fixpoint compile_fv (l:list id) : CMD ctxt :=
     (* '; store (val_of_nat 0) (local uid); *)
     (* CHKoh: is the following right? *)
     (* 'v <- compile_aexp g (ANum (Int64.repr 0%Z));  *)
-    '; store (val_of_nat 0) (local uid);
+(*    '; store (val_of_nat 0) (local uid); *)
       
     mret (update g x (local uid)) 
   end.
@@ -437,8 +491,9 @@ Definition compile (c:com) : err (toplevel_entities (list block)) :=
   '(fvs, bid, blocks) <-
           run (
             let fvs := IDSet.elements (fv c) in
-            'g <- compile_fv fvs;  
-            '; compile_com g c; 
+            '(cd, g) <- cmd_of_init (compile_fv fvs);  
+            '; compile_com g c;
+            '; inject_code cd;   
 (*            '; print_fv fvs g;  (* UNCOMMENT to enable imp state printing *) *)
             mret fvs
           )
